Prove DropUnused correct

vera/DropUnused.v
@@ -6,6 +6,7 @@ From vera Require Import Bitvector.
 From vera Require Import Common.
 Import Verilog.
 From vera Require Import VerilogSemantics.
+Import CombinationalOnly.
 
 From ExtLib Require Import Structures.Monads.
 From ExtLib Require Import Programming.Show.
@@ -48,26 +49,6 @@ Equations module_body_keep_assigns :
   }
 }.
 
-(* Definition decls_drop_vars (drop : VarSet.t) :=
- *   List.filter (fun d => negb (VarSet.mem (variable_of_decl d) drop)). *)
-
-Lemma module_body_drop_assigns_writes keep mis : 
-  LocationSet.Subset
-    (module_body_writes (snd (module_body_keep_assigns keep mis)))
-    (module_body_writes mis).
-Proof.
-  funelim (module_body_keep_assigns keep mis).
-  all: simpl.
-  - reflexivity.
-  - destruct (module_body_keep_assigns keep body) as [dropped' body'].
-    simpl in *. specialize (H tt).
-    LocationSet.setdec.
-  - destruct (module_body_keep_assigns keep body) as [dropped' body'].
-    simpl in *.
-    LocationSet.setdec.
-Qed.
-
-#[refine]
 Definition drop_unused1 {i o} (v : vmodule i o) : string + (LocationSet.t * vmodule i o) :=
   traceBracket ("Drop unused (iteration) " ++ Verilog.modName v) (
     let external_vars :=
@@ -80,9 +61,11 @@ Definition drop_unused1 {i o} (v : vmodule i o) : string + (LocationSet.t * vmod
     inr (fst result, {|
       modName := modName v;
       modBody := snd result;
+      modWfIODisjoint := modWfIODisjoint v;
+      modWfInputsNoDup := modWfInputsNoDup v;
+      modWfOutputsNoDup := modWfOutputsNoDup v;
     |})
   ).
-Proof. all: destruct v; assumption. Qed.
 
 Fixpoint drop_unused_rec {i o} (fuel : nat) (v : vmodule i o) : string + vmodule i o :=
   match fuel with
@@ -104,277 +87,117 @@ Definition drop_unused {i o} (v : vmodule i o) : string + vmodule i o :=
     drop_unused_rec (List.length (modBody v)) v
   ).
 
-(* Lemma decls_drop_internal_keep_inputs decls :
- *   Verilog.inputs_of_decls (decls_drop_vars decls) =
- *   inputs_of_decls decls.
- * Proof.
- *   funelim (Verilog.inputs_of_decls decls); simpl.
- *   - reflexivity.
- *   - rewrite Heq. simp inputs_of_decls. rewrite Heq. simpl.
- *     rewrite H. reflexivity.
- *   - rewrite Heq. simp inputs_of_decls. rewrite Heq. simpl.
- *     rewrite H. reflexivity.
- *   - rewrite Heq. simp inputs_of_decls.
- * Qed.
- * 
- * Lemma decls_drop_internal_keep_outputs decls :
- *   Verilog.outputs_of_decls (decls_drop_internal decls) =
- *   outputs_of_decls decls.
- * Proof.
- *   funelim (Verilog.outputs_of_decls decls); simpl.
- *   - reflexivity.
- *   - rewrite Heq. simp outputs_of_decls. rewrite Heq. simpl.
- *     rewrite H. reflexivity.
- *   - rewrite Heq. simp outputs_of_decls. rewrite Heq. simpl.
- *     rewrite H. reflexivity.
- *   - rewrite Heq. simp outputs_of_decls.
- * Qed.
- * 
- * Lemma module_items_sorted_permute l1 l2 body :
- *   Permutation l1 l2 ->
- *   module_items_sorted l1 body ->
- *   module_items_sorted l2 body.
- * Proof.
- *   intros Hpermutation Hsorted. revert l2 Hpermutation.
- *   induction Hsorted; constructor.
- *   - now rewrite <- Hpermutation.
- *   - now rewrite <- Hpermutation.
- *   - eapply IHHsorted.
- *     now rewrite Hpermutation.
- * Qed.
- * 
- * Global Instance Proper_module_items_sorted_permute :
- *   Proper
- *     (@Permutation _ ==> eq ==> iff)
- *     module_items_sorted.
- * Proof.
- *   intros l1 l2 Hpermutation ? _ []. split; intro H.
- *   - eapply module_items_sorted_permute; eassumption.
- *   - eapply module_items_sorted_permute; (symmetry + idtac); eassumption.
- * Qed.
- * 
- * Lemma module_items_sorted_skip l1 l2 body :
- *   disjoint l1 (module_body_reads body) ->
- *   module_items_sorted (l1 ++ l2) body ->
- *   module_items_sorted l2 body.
- * Proof.
- *   revert l1 l2.
- *   induction body; intros * Hdisjoint Hsorted; inv Hsorted; intros; constructor.
- *   - simp module_body_reads in *. disjoint_saturate.
- *     unfold list_subset, disjoint in *. rewrite Forall_forall in *.
- *     setoid_rewrite in_app_iff in H1. crush.
- *   - simp module_body_reads in *. disjoint_saturate. unpack_in.
- *     symmetry. assumption.
- *   - eapply IHbody; expect 2; cycle 1.
- *     + rewrite app_assoc.
- *       rewrite Permutation_app_comm with (l' := module_item_writes a).
- *       rewrite <- app_assoc.
- *       eassumption.
- *     + simp module_body_reads in *. disjoint_saturate.
- *       symmetry. assumption.
- * Qed.
- * 
- * Lemma module_items_sorted_add l1 l2 body :
- *   disjoint l1 (module_body_writes body) ->
- *   module_items_sorted l2 body ->
- *   module_items_sorted (l1 ++ l2) body.
- * Proof.
- *   revert l1 l2.
- *   induction body;
- *     intros * Hdisjoint Hsorted; inv Hsorted; intros; constructor;
- *     simp module_body_writes in *.
- *   - unfold list_subset, disjoint in *. rewrite Forall_forall in *.
- *     setoid_rewrite in_app_iff. crush.
- *   - unfold list_subset, disjoint in *. rewrite Forall_forall in *.
- *     setoid_rewrite in_app_iff in Hdisjoint. setoid_rewrite in_app_iff.
- *     crush.
- *   - disjoint_saturate.
- *     rewrite app_assoc.
- *     rewrite Permutation_app_comm with (l := module_item_writes a).
- *     rewrite <- app_assoc.
- *     eapply IHbody; expect 2; cycle 1.
- *     + assumption.
- *     + symmetry. assumption.
- * Qed.
- * 
- * Lemma module_items_sorted_skip1 var vars body :
- *   ~ In var (module_body_reads body) ->
- *   module_items_sorted (var :: vars) body ->
- *   module_items_sorted vars body.
- * Proof.
- *   intros.
- *   apply module_items_sorted_skip with (l1 := [var]).
- *   - constructor; crush.
- *   - crush.
- * Qed.
- * 
- * Lemma module_body_keep_vars_correct init vars inputs body :
- *   module_items_sorted inputs body ->
- *   NoDup (module_body_writes body) ->
- *   list_subset (module_body_reads body) inputs ->
- *   (exec_module_body init (module_body_keep_vars vars body))
- *     =( vars )=
- *   (exec_module_body init body).
- * Proof.
- *   revert init.
- *   funelim (module_body_keep_vars vars body).
- *   all: intros init Hsorted Hnodup Hreads.
- *   all: simp exec_module_body exec_module_item exec_statement; simpl.
- *   all: clear Heqcall.
- *   1: reflexivity.
- *   - inv Hsorted.
- *     simp module_body_writes module_item_writes statement_writes
- *          module_body_reads module_item_reads statement_reads expr_reads
- *       in *.
- *     unpack_list_subset. disjoint_saturate.
- *     apply H with (inputs:=inputs); try assumption; expect 1.
- *     eapply module_items_sorted_skip1; simpl in *; [|eassumption].
- *     unfold list_subset in *. rewrite Forall_forall in *. crush.
- *   - inv Hsorted.
- *     simp module_body_writes module_item_writes statement_writes
- *          module_body_reads module_item_reads statement_reads expr_reads
- *       in *.
- *     unpack_list_subset. disjoint_saturate.
- *     (\* edestruct (eval_expr_has_values_some _ rhs) as [x Heval_rhs]; expect 2. {
- *      *   eapply RegisterState.has_value_for_impl; [|eassumption].
- *      *   simpl. apply Forall_forall. assumption. 
- *      * } *\)
- *     (\* rewrite Heval_rhs. *\)
- *     simpl in *.
- *     rewrite H with (inputs:=inputs); try assumption; expect 2.
- *     + apply exec_module_body_change_preserve.
- *       * rewrite RegisterState.match_on_set_reg_elim; [reflexivity|].
- *         unfold list_subset in *. rewrite Forall_forall in *. crush.
- *       * rewrite RegisterState.match_on_set_reg_elim; [reflexivity|].
- *         assumption.
- *     + eapply module_items_sorted_skip1; simpl in *; [|eassumption].
- *       unfold list_subset in *. rewrite Forall_forall in *. crush.
- * Qed.
- * 
- * Lemma module_body_keep_vars_preserve init vars l inputs body :
- *   module_items_sorted inputs body ->
- *   NoDup (module_body_writes body) ->
- *   list_subset (module_body_reads body) inputs ->
- *   disjoint l (module_body_writes body) ->
- *   (exec_module_body init (module_body_keep_vars vars body))
- *     =( l )=
- *   (exec_module_body init body).
- * Proof.
- *   revert init.
- *   funelim (module_body_keep_vars vars body).
- *   all: intros init Hsorted Hnodup Hreads Hnot_written.
- *   all: simp exec_module_body exec_module_item exec_statement; simpl.
- *   all: clear Heqcall.
- *   all: try reflexivity; expect 2.
- *   - inv Hsorted.
- *     simp module_body_writes module_item_writes statement_writes
- *          module_body_reads module_item_reads statement_reads expr_reads
- *       in *.
- *     unpack_list_subset. disjoint_saturate.
- *     apply H with (inputs:=inputs); try assumption.
- *     + eapply module_items_sorted_skip1; simpl in *; [|eassumption].
- *       unfold list_subset in *. rewrite Forall_forall in *. crush.
- *     + symmetry. assumption.
- *   - inv Hsorted.
- *     simp module_body_writes module_item_writes statement_writes
- *          module_body_reads module_item_reads statement_reads expr_reads
- *       in *.
- *     unpack_list_subset. disjoint_saturate.
- *     simpl in *.
- *     erewrite H with (inputs:=inputs); try assumption; expect 3; cycle 1.
- *     + eapply module_items_sorted_skip1; simpl in *; [|eassumption].
- *       unfold list_subset in *. rewrite Forall_forall in *. crush.
- *     + symmetry. assumption.
- *     + apply exec_module_body_change_preserve.
- *       * rewrite RegisterState.match_on_set_reg_elim; [reflexivity|].
- *         unfold list_subset in *. rewrite Forall_forall in *. crush.
- *       * rewrite RegisterState.match_on_set_reg_elim; [reflexivity|].
- *         assumption.
- * Qed.
- * 
- * Lemma module_items_sorted_reads_subset inputs body :
- *   disjoint (module_body_writes body) inputs ->
- *   list_subset (module_body_reads body) inputs ->
- *   NoDup (module_body_writes body) ->
- *   module_items_sorted inputs body.
- * Proof.
- *   intros Hsubset.
- *   induction body.
- *   - constructor.
- *   - constructor;
- *       simp module_body_reads module_body_writes in *;
- *       disjoint_saturate; unpack_list_subset.
- *     + assumption.
- *     + assumption.
- *     + apply module_items_sorted_add.
- *       * unfold list_subset, disjoint in *. rewrite Forall_forall in *. crush.
- *       * apply IHbody; assumption.
- * Qed.
- * 
- * Lemma module_body_keep_vars_reads vars body :
- *   list_subset
- *     (module_body_reads (module_body_keep_vars vars body))
- *     (module_body_reads body).
- * Proof.
- *   funelim (module_body_keep_vars vars body);
- *     simp module_body_reads module_item_reads statement_reads expr_reads;
- *     try reflexivity;
- *     unfold list_subset in *; rewrite Forall_forall in *; setoid_rewrite in_app_iff;
- *     crush.
- * Qed.  
- * 
- * Lemma module_body_keep_vars_writes_subset_body vars body :
- *   list_subset
- *     (module_body_writes (module_body_keep_vars vars body))
- *     (module_body_writes body).
- * Proof.
- *   funelim (module_body_keep_vars vars body);
- *     simp module_body_writes module_item_writes statement_writes expr_reads;
- *     try reflexivity;
- *     unfold list_subset in *; rewrite Forall_forall in *; setoid_rewrite in_app_iff;
- *     crush.
- * Qed.  
- * 
- * Lemma module_body_keep_vars_writes_NoDup vars body :
- *   NoDup (module_body_writes body) ->
- *   NoDup (module_body_writes (module_body_keep_vars vars body)).
- * Proof.
- *   intros Hnodup.
- *   funelim (module_body_keep_vars vars body);
- *     simp module_body_writes module_item_writes statement_writes expr_reads in *.
- *   - simpl in *. inv Hnodup. constructor; auto.
- *     now rewrite module_body_keep_vars_writes_subset_body.
- *   - apply H. now inv Hnodup.
- * Qed.   *)
+Lemma module_body_keep_assigns_reads keep body :
+  module_body_reads body ⊆ keep ->
+  module_body_reads (snd (module_body_keep_assigns keep body)) ⊆ module_body_reads body.
+Proof.
+  funelim (module_body_keep_assigns keep body).
+  all: intros Hreads_kept.
+  all: simpl; simp exec_module_body; simpl.
+  all: clear Heqcall.
+  1: LocationSet.setdec.
+  all: rewrite (surjective_pairing (module_body_keep_assigns keep body)); simpl in *.
+  all: rewrite H by LocationSet.setdec.
+  all: LocationSet.setdec.
+Qed.
+
+Lemma module_body_keep_assigns_spec keep init body :
+  module_body_reads body ⊆ keep ->
+  exec_module_body init (snd (module_body_keep_assigns keep body)) =( keep )= exec_module_body init body.
+Proof.
+  intros Hreads_kept.
+  funelim (module_body_keep_assigns keep body).
+  all: simpl; simp exec_module_body; simpl.
+  all: clear Heqcall.
+  1: reflexivity.
+  all: rewrite (surjective_pairing (module_body_keep_assigns keep body)); simpl in *.
+  all: simp exec_module_body exec_module_item exec_statement; simpl in *.
+  2: apply H; LocationSet.setdec.
+  apply LocationSet.disjoint_spec in Heq.
+  rewrite Facts.exec_module_body_change_preserve.
+  - apply H; LocationSet.setdec.
+  - symmetry. apply Facts.set_target_preserve.
+    rewrite module_body_keep_assigns_reads by LocationSet.setdec.
+    LocationSet.setdec.
+  - symmetry. apply Facts.set_target_preserve.
+    LocationSet.setdec.
+Qed.
 
 Import ExactEquivalence.
+
+Lemma module_body_keep_assigns_sorted keep vars body :
+  module_body_reads body ⊆ keep ->
+  module_items_sorted vars body ->
+  module_items_sorted vars (snd (module_body_keep_assigns keep body)).
+Proof.
+  funelim (module_body_keep_assigns keep body).
+  all: clear Heqcall.
+  all: intros Hreads Hsorted.
+  1: solve [constructor].
+  all: cbn in *.
+  all: rewrite (surjective_pairing (module_body_keep_assigns keep body)); simpl.
+  all: inv Hsorted.
+  - apply LocationSet.disjoint_spec in Heq.
+    eapply module_items_sorted_skip with (vars_skip := assign_target_writes lhs).
+    + rewrite module_body_keep_assigns_reads. all: LocationSet.setdec.
+    + apply H. all: intuition LocationSet.setdec.
+  - constructor; try assumption; expect 1.
+    apply H. all: intuition LocationSet.setdec.
+Qed.
+
+Lemma drop_unused1_transfer_sorted {i o} dropped (v1 v2 : vmodule i o) :
+  drop_unused1 v1 = inr (dropped, v2) ->
+  vmodule_sorted v1 ->
+  vmodule_sorted v2.
+Proof.
+  intros Hdrop Hsorted.
+  destruct v1, v2.
+  unfold drop_unused1 in Hdrop.
+  simpl in *.
+  monad_inv.
+  apply module_body_keep_assigns_sorted.
+  - LocationSet.setdec.
+  - exact Hsorted.
+Qed.
+
+Lemma drop_unused1_exact_equivalence {i o} dropped (v1 v2 : vmodule i o) :
+  vmodule_sorted v1 ->
+  drop_unused1 v1 = inr (dropped, v2) ->
+  v1 ~~~ v2.
+Proof.
+  intros Hsorted H.
+  apply exact_by_output_equality.
+  unfold run_vmodule, mk_initial_state.
+  intros.
+  rewrite sort_module_items_stable by exact Hsorted.
+  rewrite sort_module_items_stable by (eapply drop_unused1_transfer_sorted; eassumption).
+  destruct v1, v2. unfold drop_unused1 in *. simpl in *.
+  monad_inv.
+  symmetry.
+  eapply RegisterState.match_on_subset; cycle 1.
+  - apply module_body_keep_assigns_spec. LocationSet.setdec.
+  - LocationSet.setdec.
+Qed.
+
+#[local] Opaque drop_unused1.
 
 Theorem drop_unused_exact_equivalence {i o} (v1 v2 : vmodule i o) :
   drop_unused v1 = inr v2 ->
   v1 ~~~ v2.
-Proof. Admitted.
-(*   intros H.
- *   unfold drop_internal in H.
- *   monad_inv.
- *   apply exact_by_output_equality.
- *   - symmetry. apply decls_drop_internal_keep_inputs.
- *   - symmetry. apply decls_drop_internal_keep_outputs.
- *   - intros *.
- *     unfold run_vmodule in *.
- *     unfold module_inputs, module_outputs in *; simpl in *.
- *     rewrite ! sort_module_items_stable in *; expect 3; cycle 1.
- *     + rewrite decls_drop_internal_keep_inputs.
- *       apply module_items_sorted_reads_subset.
- *       * rewrite module_body_keep_vars_writes_subset_body.
- *         symmetry. assumption.
- *       * rewrite module_body_keep_vars_reads.
- *         assumption.
- *       * apply module_body_keep_vars_writes_NoDup. assumption.
- *     + assumption.
- *     + unfold mk_initial_state, module_inputs in *; simpl in *.
- *       rewrite decls_drop_internal_keep_inputs in *.
- *       symmetry.
- *       RegisterState.unpack_match_on.
- *       * eapply module_body_keep_vars_preserve; try eassumption.
- *       * eapply module_body_keep_vars_correct; eassumption.
- * Qed. *)
+Proof.
+  unfold drop_unused. simpl.
+  generalize (Datatypes.length (modBody v1)). intro fuel.
+  intros H.
+  monad_inv.
+  revert v1 v2 m H.
+  induction fuel.
+  all: intros.
+  all: simpl in H.
+  all: monad_inv.
+  - reflexivity.
+  - eapply drop_unused1_exact_equivalence; eassumption.
+  - transitivity v.
+    + eapply drop_unused1_exact_equivalence; eassumption.
+    + apply IHfuel; [|eassumption].
+      eapply drop_unused1_transfer_sorted; eassumption.
+Qed.
